tests/lean/run/binrel.lean
@@ -1,35 +1,35 @@
 def ex1 (x y : Nat) (i j : Int) :=
-  binrel% Less x i
+  binrel% LT.lt x i
 
 def ex2 (x y : Nat) (i j : Int) :=
-  binrel% Less i x
+  binrel% LT.lt i x
 
 def ex3 (x y : Nat) (i j : Int) :=
-  binrel% Less (i + 1) x
+  binrel% LT.lt (i + 1) x
 
 def ex4 (x y : Nat) (i j : Int) :=
-  binrel% Less i (x + 1)
+  binrel% LT.lt i (x + 1)
 
 def ex5 (x y : Nat) (i j : Int) :=
-  binrel% Less i (x + y)
+  binrel% LT.lt i (x + y)
 
 def ex6 (x y : Nat) (i j : Int) :=
-  binrel% Less (i + j) (x + 0)
+  binrel% LT.lt (i + j) (x + 0)
 
 def ex7 (x y : Nat) (i j : Int) :=
-  binrel% Less (i + j) (x + i)
+  binrel% LT.lt (i + j) (x + i)
 
 def ex8 (x y : Nat) (i j : Int) :=
-  binrel% Less (i + 0) (x + i)
+  binrel% LT.lt (i + 0) (x + i)
 
 def ex9 (n : UInt32) :=
-  binrel% Less n 0xd800
+  binrel% LT.lt n 0xd800
 
 def ex10 (x : Lean.Syntax) : Bool :=
   x.getArgs.all (binrel% BEq.beq ·.getKind `foo)
 
 def ex11 (xs : Array (Nat × Nat)) :=
-  let f a b := binrel% Less a.1 b.1
+  let f a b := binrel% LT.lt a.1 b.1
   f xs[1] xs[2]
 
 def ex12 (i j : Int) :=
